ListsOp/Forall_ZopList.v
@@ -1,4 +1,5 @@
 Require Import stdpp.prelude.
+Require Import ssreflect.
 From Tweetnacl Require Export ListsOp.Zipp.
 From Tweetnacl Require Export ListsOp.ZunopList.
 From Tweetnacl Require Import Libs.Export.
