Low/Inv25519_gen.v
@@ -1,4 +1,5 @@
 Require Import Tweetnacl.Libs.Export.
+Require Import ssreflect.
 Require Import Recdef.
 (*
 Require Import Tweetnacl.Libs.HeadTailRec.
