Low/Reduce_by_P_compose_1.v
@@ -1,0 +1,18 @@
+From Tweetnacl Require Import Libs.Export.
+From Tweetnacl Require Import ListsOp.Export.
+From Tweetnacl Require Import Low.Reduce_by_P_compose_step.
+
+From stdpp Require Import prelude.
+Require Import Recdef.
+
+Open Scope Z.
+
+Definition subst_0xffff t := t - 65535.
+
+Definition sub_step_1 (a:Z) (m t:list Z) : list Z :=
+    let t' := nth (Z.to_nat a) t 0 in
+      (upd_nth (Z.to_nat a) m (subst_0xffff t')).
+
+
+
+Close Scope Z.
