Low/Reduce_by_P_compose_2.v
@@ -1,0 +1,150 @@
+From Tweetnacl Require Import Libs.Export.
+From Tweetnacl Require Import ListsOp.Export.
+From Tweetnacl Require Import Low.Reduce_by_P_compose_step.
+
+(* From Tweetnacl Require Import Mid.SubList. *)
+(* From Tweetnacl Require Import Low.Get_abcdef. *)
+(* From Tweetnacl Require Import Low.GetBit_pack25519. *)
+(* From Tweetnacl Require Import Low.Sel25519. *)
+(* From Tweetnacl Require Import Low.Constant. *)
+(* From Tweetnacl Require Import Libs.Lists_extended.
+From Tweetnacl Require Import Libs.List_Ltac.
+From Tweetnacl Require Import Libs.LibTactics_SF.
+From Tweetnacl Require Import Libs.LibTactics.
+ *)
+ From stdpp Require Import prelude.
+Require Import Recdef.
+Require Import ssreflect.
+Open Scope Z.
+
+Definition subst_c t m := t - (Z.land (Z.shiftr m 16) 1).
+
+Definition sub_step_2 (a:Z) (m:list Z) : list Z :=
+    let m' := nth (Z.to_nat (a - 1)) m 0 in
+    let t' := nth (Z.to_nat a) m 0 in
+      upd_nth (Z.to_nat (a-1)) (upd_nth (Z.to_nat a) m (subst_c t' m')) (mod0xffff m').
+
+Lemma sub_step_2_Z_inv : forall a m,
+0 < a < Zlength m ->
+- 2^16 <= nth (Z.to_nat (a - 1)) m 0 <= 0 ->
+ZofList 16 (sub_step_2 a m) = ZofList 16 m.
+Proof.
+intros a m Hm Hbm.
+rewrite /sub_step_2 /mod0xffff /subst_c.
+rewrite ?ZofList_upd_nth_Zlength.
+5: rewrite upd_nth_Zlength.
+3,5,6: rewrite Z2Nat.id.
+all: try omega.
+rewrite Zplus_assoc_reverse.
+match goal with
+  | [ |- _ + ?A = _ ] => replace A with 0
+end.
+symmetry.
+apply Zplus_0_r_reverse.
+replace (16 * Z.to_nat a) with (16 * Z.to_nat (a - 1) + 16).
+2: rewrite ?Z2Nat.id ; omega.
+rewrite Z.pow_add_r.
+2: rewrite ?Z2Nat.id.
+2,3,4 : omega.
+rewrite Zmult_assoc_reverse.
+rewrite Zred_factor4.
+symmetry ; rewrite Z.mul_comm; apply Z_eq_mult.
+rewrite upd_nth_diff_Zlength.
+2,3: rewrite Z2Nat.id.
+all: try omega.
+2: intro H; apply (f_equal Z.of_nat) in H; rewrite ?Z2Nat.id in H; omega.
+replace (2 ^ 16 * (- nth (Z.to_nat a) m 0 + (nth (Z.to_nat a) m 0 - Z.land (nth (Z.to_nat (a - 1)) m 0 ≫ 16) 1)) + (- nth (Z.to_nat (a - 1)) m 0 + Z.land (nth (Z.to_nat (a - 1)) m 0) 65535)) with 
+(2^16 * (nth (Z.to_nat a) m 0) - 2^16 * (nth (Z.to_nat a) m 0) - 2^16 * (Z.land (nth (Z.to_nat (a - 1)) m 0 ≫ 16) 1) + Z.land (nth (Z.to_nat (a - 1)) m 0) 65535 - nth (Z.to_nat (a - 1)) m 0).
+2: ring.
+replace (2 ^ 16 * nth (Z.to_nat a) m 0 - 2 ^ 16 * nth (Z.to_nat a) m 0) with 0 by omega.
+change 65535 with (Z.ones 16).
+change 1 with (Z.ones 1).
+rewrite ?Z.land_ones.
+change (Z.ones 1) with 1.
+2,3: omega.
+match goal with
+| [ |- ?A = _ ] => replace A with (nth (Z.to_nat (a - 1)) m 0 `mod` 2 ^ 16 - (2 ^ 16 * (nth (Z.to_nat (a - 1)) m 0 ≫ 16) `mod` 2 ^ 1 + nth (Z.to_nat (a - 1)) m 0))
+end.
+2: omega.
+symmetry.
+apply Zplus_minus_eq.
+rewrite -Zplus_0_r_reverse.
+rewrite Zmod_eq.
+2: apply pown0 ; omega.
+remember (nth (Z.to_nat (a - 1)) m 0) as n.
+clear Hm Heqn ; clears.
+rewrite Z.shiftr_div_pow2.
+2: omega.
+assert(Hn: n = 0 \/ n < 0) by omega.
+destruct Hn.
+subst n ; reflexivity.
+
+assert(n `div` 2 ^ 16 = -1).
+  assert(n `div` 2 ^ 16 < 0).
+    apply Z.div_lt_upper_bound ; omega.
+  assert((- 2 ^ 16) `div` 2 ^ 16 <= n `div` 2 ^ 16).
+    apply Z_div_le; try omega.
+  change ((- 2 ^ 16) `div` 2 ^ 16) with (-1) in H1.
+  omega.
+rewrite H0.
+change ((-1) `mod` 2 ^ 1 ) with 1.
+ring.
+Qed.
+
+Lemma sub_fn_rev_s_sub_step_2_inv : forall a m,
+  0 < a < 16 ->
+  Zlength m = 16 ->
+  Forall (fun x => - 2^16 <= x <= 0) (take 15 m) ->
+  ZofList 16 (sub_fn_rev_s sub_step_2 a m) = ZofList 16 m.
+Proof.
+intros a m Ha Hm Hb.
+(* assert_gen_hyp_ H a 15 14 ; try omega. *)
+assert(Hbound: forall a, 0 < a /\ a < 16 -> - 2^16 <= nth (Z.to_nat (a - 1)) m 0 <= 0).
+{
+  intros x Hx.
+  replace(nth (Z.to_nat (x - 1)) m 0) with (nth (Z.to_nat (x - 1)) (take 15 m) 0).
+  apply Forall_nth_d.
+  compute ; split ; discriminate.
+  assumption.
+  apply nth_take_full.
+  change 15%nat with (Z.to_nat 15).
+  apply Z2Nat.inj_lt ; omega.
+}
+assert(H1: ℤ16.lst sub_fn_rev_s sub_step_2 1 m = ℤ16.lst m).
+  rewrite sub_fn_rev_s_1 ; reflexivity.
+assert(H2: ℤ16.lst sub_fn_rev_s sub_step_2 2 m = ℤ16.lst m).
+  rewrite sub_fn_rev_s_n ; try apply sub_step_2_Z_inv ; try apply Hbound ; try omega.
+assert(H3: ℤ16.lst sub_fn_rev_s sub_step_2 3 m = ℤ16.lst m).
+  admit.
+Admitted.
+(* assert(H4: ℤ16.lst sub_fn_rev_s sub_step_2 4 m = ℤ16.lst m).
+assert(H5: ℤ16.lst sub_fn_rev_s sub_step_2 5 m = ℤ16.lst m).
+assert(H6: ℤ16.lst sub_fn_rev_s sub_step_2 6 m = ℤ16.lst m).
+assert(H7: ℤ16.lst sub_fn_rev_s sub_step_2 7 m = ℤ16.lst m).
+assert(H8: ℤ16.lst sub_fn_rev_s sub_step_2 8 m = ℤ16.lst m).
+assert(H9: ℤ16.lst sub_fn_rev_s sub_step_2 9 m = ℤ16.lst m).
+assert(H10: ℤ16.lst sub_fn_rev_s sub_step_2 10 m = ℤ16.lst m).
+assert(H11: ℤ16.lst sub_fn_rev_s sub_step_2 11 m = ℤ16.lst m).
+assert(H12: ℤ16.lst sub_fn_rev_s sub_step_2 12 m = ℤ16.lst m).
+assert(H13: ℤ16.lst sub_fn_rev_s sub_step_2 13 m = ℤ16.lst m).
+assert(H14: ℤ16.lst sub_fn_rev_s sub_step_2 14 m = ℤ16.lst m).
+assert(H15: ℤ16.lst sub_fn_rev_s sub_step_2 15 m = ℤ16.lst m).
+destruct H ; [subst a|].
+reflexivity.
+destruct H ; [subst a|].
+
+destruct a.
+reflexivity.
+reflex
+induction a.
+rewrite 
+ *)
+
+
+
+
+
+
+
+Close Scope Z.
+
