Low/Reduce_by_P_compose_step.v
@@ -1,0 +1,224 @@
+From Tweetnacl Require Import Libs.Export.
+From Tweetnacl Require Import ListsOp.Export.
+(* From Tweetnacl Require Import Mid.SubList. *)
+(* From Tweetnacl Require Import Low.Get_abcdef. *)
+(* From Tweetnacl Require Import Low.GetBit_pack25519. *)
+(* From Tweetnacl Require Import Low.Sel25519. *)
+(* From Tweetnacl Require Import Low.Constant. *)
+(* From Tweetnacl Require Import Libs.Lists_extended.
+From Tweetnacl Require Import Libs.List_Ltac.
+From Tweetnacl Require Import Libs.LibTactics_SF.
+From Tweetnacl Require Import Libs.LibTactics.
+ *)
+From stdpp Require Import prelude.
+Require Import Recdef.
+
+(*
+sv pack25519(u8 *o,const gf n)
+{
+  int i,j,b;
+  gf m,t;
+  FOR(i,16) t[i]=n[i];
+  car25519(t);
+  car25519(t);
+  car25519(t);
+  FOR(j,2) {
+    m[0]=t[0]-0xffed;
+
+    for(i=1;i<15;i++) {
+      m[i]=t[i]-0xffff-((m[i-1]>>16)&1);
+      m[i-1]&=0xffff;
+    }
+
+    for(i=1;i<15;i++) {
+      m[i]=t[i];
+    }
+    for(i=1;i<15;i++) {
+      m[i]=m[i]-((m[i-1]>>16)&1);
+      m[i-1]&=0xffff;
+    }
+
+
+
+
+    m[15]=t[15]-0x7fff-((m[14]>>16)&1);
+    b=(m[15]>>16)&1;
+    m[14]&=0xffff;
+    sel25519(t,m,1-b);
+  }
+  FOR(i,16) {
+    o[2*i]=t[i]&0xff;
+    o[2*i+1]=t[i]>>8;
+  }
+}
+*)
+
+Open Scope Z.
+(*
+0xffff = 65535
+0xffed = 65517
+0x7fff = 32767
+*)
+
+(* Definition subst_0xffed t := t - 65517. *)
+Definition subst_0xffffc t m := t - 65535 - (Z.land (Z.shiftr m 16) 1).
+(* Definition subst_0xffff t := t - 65535. *)
+(* Definition subst_0x7fffc t m := t - 32767 - (Z.land (Z.shiftr m 16) 1). *)
+(* Definition subst_0x7fff t := t - 32767. *)
+(* Definition subst_c t m := t - (Z.land (Z.shiftr m 16) 1). *)
+Definition mod0xffff m := Z.land m 65535.
+
+Definition sub_step (a:Z) (m t:list Z) : list Z :=
+    let m' := nth (Z.to_nat (a - 1)) m 0 in
+    let t' := nth (Z.to_nat a) t 0 in
+      upd_nth (Z.to_nat (a-1)) (upd_nth (Z.to_nat a) m (subst_0xffffc t' m')) (mod0xffff m').
+
+Lemma nth_i_1_substep: forall i m t, 
+  Zlength m = Zlength t ->
+  0 < i < Zlength m ->
+  nth (Z.to_nat (i - 1)) (sub_step i m t) 0 = mod0xffff (nth (Z.to_nat (i - 1)) m 0).
+Proof.
+  intros i m t Hmt Him.
+  unfold sub_step, mod0xffff.
+  rewrite upd_nth_same_Zlength ; try reflexivity.
+  split ; try omega ; rewrite upd_nth_Zlength ; rewrite Z2Nat.id ; try omega.
+Qed.
+
+Lemma nth_i_substep: forall i m t, 
+  Zlength m = Zlength t ->
+  0 < i < Zlength m ->
+  nth (Z.to_nat (i)) (sub_step i m t) 0 = subst_0xffffc (nth (Z.to_nat i) t 0) (nth (Z.to_nat (i - 1)) m 0).
+Proof.
+  intros i m t Hmt Him.
+  unfold sub_step.
+  rewrite upd_nth_diff_Zlength.
+  2: split ; try omega ; rewrite upd_nth_Zlength ; rewrite Z2Nat.id ; try omega.
+  2: split ; try omega ; rewrite upd_nth_Zlength ; rewrite Z2Nat.id ; try omega.
+  2: intros H ; apply (f_equal Z.of_nat) in H ; rewrite ?Z2Nat.id in H ; omega.
+  rewrite upd_nth_same_Zlength ; try reflexivity.
+  rewrite Z2Nat.id ; try omega.
+Qed.
+
+(* Definition of the for loop : 1 -> 15 *)
+Function sub_fn_rev {A} (f:Z -> list A -> list A -> list A) (a:Z) (m t: list A) {measure Z.to_nat a} : (list A) :=
+  if (a <=? 1)
+    then m
+    else
+      let prev := sub_fn_rev f (a - 1) m t in 
+        f (a - 1) prev t.
+Proof. intros. apply Z2Nat.inj_lt ; rewrite Z.leb_gt in teq; omega. Defined.
+
+Arguments sub_fn_rev [_] _ _ _.
+
+Lemma sub_fn_rev_1 : forall A f (m t:list A),
+  sub_fn_rev f 1 m t = m.
+Proof. intros. reflexivity. Qed.
+
+Lemma sub_fn_rev_n : forall A f (m t:list A) a,
+  1 < a ->
+  sub_fn_rev f a m t = f (a - 1) (sub_fn_rev f (a - 1) m t) t.
+Proof. intros. rewrite sub_fn_rev_equation.
+destruct (a <=? 1) eqn:Eq.
+apply Zle_bool_imp_le in Eq; omega.
+reflexivity.
+Qed.
+
+(* Definition of the for loop : 1 -> 15 *)
+Function sub_fn_rev_s {A} (f:Z -> list A -> list A) (a:Z) (m: list A) {measure Z.to_nat a} : (list A) :=
+  if (a <=? 1)
+    then m
+    else
+      let prev := sub_fn_rev_s f (a - 1) m in 
+        f (a - 1) prev.
+Proof. intros. apply Z2Nat.inj_lt ; rewrite Z.leb_gt in teq; omega. Defined.
+
+Arguments sub_fn_rev_s [_] _ _ _.
+
+Lemma sub_fn_rev_s_1 : forall A f (m: list A),
+  sub_fn_rev_s f 1 m = m.
+Proof. intros. reflexivity. Qed.
+
+Lemma sub_fn_rev_s_n : forall A a (m: list A) f,
+  1 < a ->
+  sub_fn_rev_s f a m = f (a - 1) (sub_fn_rev_s f (a - 1) m).
+Proof. intros. rewrite sub_fn_rev_s_equation.
+destruct (a <=? 1) eqn:Eq.
+apply Zle_bool_imp_le in Eq; omega.
+reflexivity.
+Qed.
+
+Lemma nth_i_1_substep_bounds: forall i m t,
+  Zlength m = Zlength t ->
+  0 < i < Zlength m ->
+  0 <= nth (Z.to_nat (i - 1)) (sub_step i m t) 0 < 2^16.
+Proof.
+  intros.
+  rewrite nth_i_1_substep ; auto.
+  unfold mod0xffff.
+  change 65535 with (Z.ones 16).
+  rewrite Z.land_ones ; try omega.
+  apply Z_mod_lt.
+  apply pown0 ; omega.
+Qed.
+
+Lemma nth_i_substep_bounds: forall i m t,
+  Zlength m = Zlength t ->
+  0 < i < Zlength m ->
+  Forall (fun x => 0 <= x < 2^16) t ->
+  -2^16 <= nth (Z.to_nat i) (sub_step i m t) 0 <= 0.
+Proof.
+intros i m t Hmt Him HPt.
+rewrite nth_i_substep ; auto.
+unfold subst_0xffffc.
+assert(HP0: 0 ≤ 0 ∧ 0 < 2 ^ 16) by (split ; try omega ; apply Z.gt_lt ; apply pown0 ; omega).
+assert(0 ≤ (nth (Z.to_nat i) t 0) ∧ (nth (Z.to_nat i) t 0) < 2 ^ 16).
+apply Forall_nth_d; assumption.
+assert(HZlandminmax:= and_0_or_1 (nth (Z.to_nat (i - 1)) m 0 ≫ 16)).
+assert(HZland: Z.land (nth (Z.to_nat (i - 1)) m 0 ≫ 16) 1 = 0 \/ Z.land (nth (Z.to_nat (i - 1)) m 0 ≫ 16) 1 = 1) by omega.
+destruct HZland as [HZland|HZland]; rewrite HZland.
+all: change (2^16) with 65536 in * ; omega.
+Qed.
+
+Lemma subst_select_step_Zlength : forall i m t,
+  0 < i < Zlength m->
+  Zlength (sub_step i m t) = Zlength m.
+Proof.
+  intros.
+  unfold sub_step.
+  assert(0 < Z.to_nat i /\ Z.to_nat i < Zlength m) by (rewrite ?Z2Nat.id ; omega).
+  assert(Z.of_nat (Z.to_nat (i - 1)) = (Z.of_nat (Z.to_nat i)) - 1) by (rewrite ?Z2Nat.id ; omega).
+  repeat rewrite ?upd_nth_Zlength ; try omega.
+Qed.
+
+Local Lemma sub_fn_rev_Zlength_ind_step : forall i m t,
+  0 < i < Zlength m ->
+  Zlength (sub_fn_rev sub_step i m t) = Zlength m ->
+  Zlength (sub_fn_rev sub_step (i+1) m t) = Zlength m.
+Proof.
+intros i m t Him Hind.
+rewrite sub_fn_rev_equation.
+flatten.
+replace ( i + 1 - 1) with i by omega.
+rewrite <- Hind.
+apply subst_select_step_Zlength.
+rewrite Hind.
+assumption.
+Qed.
+
+Lemma sub_fn_rev_Zlength : forall i m t,
+  Zlength m = 16 ->
+  0 < i < Zlength m ->
+  Zlength (sub_fn_rev sub_step i m t) = Zlength m.
+Proof.
+intros.
+change(Zlength (sub_fn_rev sub_step i m t) = Zlength m) with
+  ((fun x => Zlength (sub_fn_rev sub_step x m t) = Zlength m) i).
+apply P016_impl.
+by rewrite sub_fn_rev_1.
+intros ; apply sub_fn_rev_Zlength_ind_step.
+2: apply H2.
+all: omega.
+Qed.
+
+
+Close Scope Z.
