Low/S.v
@@ -1,5 +1,6 @@
 Require Import Tweetnacl.Libs.Export.
 Require Export Tweetnacl.Low.M.
+Require Import ssreflect.
 
 Definition Sq (a : list Z) : list Z := M a a.
 
