Low/ScalarMult_gen.v
@@ -1,3 +1,4 @@
+Require Import ssreflect.
 (*
 int crypto_scalarmult(u8 *q,const u8 *n,const u8 *p)
 {
