Low/ScalarMult_rev_rec_gen.v
@@ -1,3 +1,4 @@
+Require Import ssreflect.
 Require Import Tweetnacl.Libs.Export.
 Require Import Tweetnacl.Libs.HeadTailRec.
 Require Import Tweetnacl.Low.Get_abcdef.
