Mid/ZCarry.v
@@ -2,6 +2,7 @@ From Tweetnacl Require Import Libs.Export.
 From Tweetnacl Require Import Mid.Reduce.
 From Tweetnacl Require Import Mid.Carry.
 From Tweetnacl Require Import Low.Car25519.
+Require Import ssreflect.
 Require Import Nsatz.
 Require Import Psatz.
 
